theories/util/types.v
@@ -22,7 +22,7 @@ Infix "^++" := tapp (at level 60, right associativity).
 Fixpoint tnth B As (i: nat) := match As with
   ^[] => B | A ^:: As' => match i with 0 => A | S j => tnth B As' j end end.
 
-Notation tnthe := (tnth Empty_set).
+Notation tnthe := (tnth ∅).
 
 (** * Heterogeneous List *)
 
@@ -79,7 +79,7 @@ Proof. move=> Imp. elim; constructor; by [apply Imp|]. Qed.
 Lemma HForall_nth {F B As} (Φ: ∀A, F A → Prop) (y: _ B) (xl: _ As) i :
   Φ _ y → HForall Φ xl → Φ _ (hnth y xl i).
 Proof.
-  move=> ? All. move: i. elim: All=> /=[|> ???]; by [move=> ?|case=> [|?]].
+  move=> ? All. move: i. elim All=> /=[|> ???]; by [move=> ?|case=> [|?]].
 Qed.
 
 Inductive HForall2 {F G} (Φ: ∀A, F A → G A → Prop)
@@ -106,7 +106,7 @@ Qed.
 Lemma HForall2_nth {F G B As} (Φ: ∀A, F A → G A → Prop) (x y: _ B) (xl yl: _ As) i :
   Φ _ x y → HForall2 Φ xl yl → Φ _ (hnth x xl i) (hnth y yl i).
 Proof.
-  move=> ? All. move: i. elim: All=> /=[|> ???]; by [move=> ?|case=> [|?]].
+  move=> ? All. move: i. elim All=> /=[|> ???]; by [move=> ?|case=> [|?]].
 Qed.
 
 Global Instance HForall2_reflexive {F As} (R: ∀A, F A → F A → Prop) :
@@ -177,7 +177,7 @@ Fixpoint hlist_to_plist {F As} (xl: hlist F As) : plist F As :=
 
 Fixpoint plist2 (F: Type → Type → Type) As Bs : Type :=
   match As, Bs with ^[], ^[] => :1 |
-    A ^:: As', B ^:: Bs' => F A B :* plist2 F As' Bs' | _, _ => Empty_set end.
+    A ^:: As', B ^:: Bs' => F A B :* plist2 F As' Bs' | _, _ => ∅ end.
 
 Fixpoint p2map {F G As Bs} (f: ∀A B, F A B → G A B) : plist2 F As Bs → plist2 G As Bs :=
   match As, Bs with ^[], ^[] => id
@@ -266,7 +266,7 @@ Lemma HForallZip_nth {F G H C D As Bs} (Φ: ∀A B, F A → G B → H A B → Pr
   (x: _ C) (y: _ D) z (xl: _ As) (yl: _ Bs) zl i :
   Φ _ _ x y z → HForallZip Φ xl yl zl → Φ _ _ (hnth x xl i) (hnth y yl i) (p2nth z zl i).
 Proof.
-  move=> ? All. move: i. elim: All=> /=[|> ???]; by [move=> ?|case=> [|?]].
+  move=> ? All. move: i. elim All=> /=[|> ???]; by [move=> ?|case=> [|?]].
 Qed.
 
 (** * Sum *)
